## "Complete The Square" method

First we need to write the Quadratic Equation:

$$ax^2+bx+c = 0$$

We should assume that $a$ is not 0 in this case, and divide both sides by it, giving us:

$$x^2+\frac{b}{a}x+\frac{c}{a} = 0$$

Next step is to subtract $\frac{c}{a}$ from both sides, giving us:

$$x^2+\frac{b}{a}x = -\frac{c}{a}$$

Next, to actually use "Complete The Square" method, we have to add a term such that $x^2 + 2yx + y^2$ gets simplified to a complete square $(x + y)^2$, and that term in this case is $(\frac{b}{2a})^2$:

$$x^2+2\frac{b}{2a}x+(\frac{b}{2a})^2 = (\frac{b}{2a})^2 - \frac{c}{a}$$

We further simplify it:

$$(x+\frac{b}{2a})^2 = (\frac{b}{2a})^2 - \frac{c}{a}$$
$$(x+\frac{b}{2a})^2 = \frac{b^2}{4a^2} - \frac{c}{a}$$
$$(x+\frac{b}{2a})^2 = \frac{b^2 - 2ac}{4a^2}$$

Taking the square root on both sides

$$x+\frac{b}{2a} = \frac{\pm \sqrt{b^2 - 2ac}}{2a}$$

Subtracting $\frac{b}{2a}$ from both sides:

$$x = \frac{-b \pm \sqrt{b^2 - 2ac}}{2a}$$

And there we have it! only $x$ on the left side and on the right side are the coefficients of $x$
